iris_heap_lang/lib/assert.v
@@ -10,7 +10,7 @@ Definition assert : val :=
 Notation "'assert:' e" := (assert (λ: <>, e)%E) (at level 99) : expr_scope.
 Notation "'assert:' e" := (assert (λ: <>, e)%V) (at level 99) : val_scope.
 
-Lemma twp_assert `{!heapG Σ} E (Φ : val → iProp Σ) e :
+Lemma twp_assert `{!heapGS Σ} E (Φ : val → iProp Σ) e :
   WP e @ E [{ v, ⌜v = #true⌝ ∧ Φ #() }] -∗
   WP (assert: e)%V @ E [{ Φ }].
 Proof.
@@ -18,7 +18,7 @@ Proof.
   wp_smart_apply (twp_wand with "HΦ"). iIntros (v) "[% ?]"; subst. by wp_if.
 Qed.
 
-Lemma wp_assert `{!heapG Σ} E (Φ : val → iProp Σ) e :
+Lemma wp_assert `{!heapGS Σ} E (Φ : val → iProp Σ) e :
   WP e @ E {{ v, ⌜v = #true⌝ ∧ ▷ Φ #() }} -∗
   WP (assert: e)%V @ E {{ Φ }}.
 Proof.
