iris_heap_lang/total_adequacy.v
@@ -4,8 +4,8 @@ From iris.heap_lang Require Export adequacy.
 From iris.heap_lang Require Import proofmode notation.
 From iris.prelude Require Import options.
 
-Definition heap_total Σ `{!heapPreG Σ} s e σ φ :
-  (∀ `{!heapG Σ}, ⊢ inv_heap_inv -∗ WP e @ s; ⊤ [{ v, ⌜φ v⌝ }]) →
+Definition heap_total Σ `{!heapGpreS Σ} s e σ φ :
+  (∀ `{!heapGS Σ}, ⊢ inv_heap_inv -∗ WP e @ s; ⊤ [{ v, ⌜φ v⌝ }]) →
   sn erased_step ([e], σ).
 Proof.
   intros Hwp; eapply (twp_total _ _); iIntros (?) "".
@@ -16,5 +16,5 @@ Proof.
   iExists
     (λ σ κs _, (gen_heap_interp σ.(heap) ∗ proph_map_interp κs σ.(used_proph_id))%I),
     (λ _, True%I); iFrame.
-  iApply (Hwp (HeapG _ _ _ _ _)). done.
+  iApply (Hwp (HeapGS _ _ _ _ _)). done.
 Qed.
